update

code/tests/Hacl.Test.Circuits.fst
@@ -6,37 +6,102 @@ open FStar.Tactics
 
 module UI=FStar.UInt
 
-let m:pos = 1
-let p:pos = 4
+let m:pos = 8
+let p:pos = 16
 
 let circ : circuit m p =
-  let rec aux (i:nat) : circuit m (i+1) =
-    if i=0 then
-      Cons Empty (Input 0)
-    else
-      Cons (aux (i-1)) (Xor (i-1) (i-1))
-  in
-  aux (p-1)
+  normalize_term(
+    let rec aux (i:nat) : circuit m (i+1) =
+      if i=0 then
+        Cons Empty (Input 0)
+      else
+        Cons (aux (i-1)) (Xor (i-1) (i-1))
+    in
+    aux (p-1)
+  )
+
+
+open FStar.HyperStack.All
+open FStar.HyperStack
+open FStar.HyperStack.ST
+module B=Lib.Bitmap
+module IT=Lib.IntTypes
+
+let lN = B.uN IT.U64 IT.SEC 64
+
+let pp (_:unit) : Tac unit =
+  norm [ delta_only [`%m; `%p] ];
+  norm [ delta_only [`%circuit_impl] ];
+
+  // unroll circuit
+  norm [ zeta; delta_only [`%rev; `%circ]; iota ];
+
+  // normalize initial acc
+  norm [ zeta; delta_only [`%xNxM_empty; `%xNxM_mk]; iota; primops ];
+
+  let _ = repeatn (p+1) (fun _ ->
+    norm [ zeta; delta_only [`%circuit_impl_aux] ];
+    norm [ zeta; delta_only [`%index]; iota; primops ];
+    ()
+  ) in
+
+  norm [ delta_only
+    [ `%lN
+    ; `%Mkfoo?.t
+    ; `%Mkbar?.xN
+    ; `%Lib.Bitmap.uN
+    ; `%Mkbar
+    ; `%Mkbar?.xor_
+    ]
+  ];
+
+  dump "";
+  trefl ()
+
+[@@postprocess_with pp]
+let test2 (x:xNxM lN.xN m) :
+  Stack (xNxM lN.xN p)
+    (requires fun _ -> True)
+    (ensures fun _ _ _ -> True)
+  =
+  circuit_impl circ lN x
+
+let pp' (_:unit) : Tac unit =
+  norm [ delta_only [`%test2] ];
+  norm [ delta_only
+    [ `%lN
+    ; `%Mkfoo?.t
+    ; `%Mkbar?.xN
+    ; `%Lib.Bitmap.uN
+    ; `%Mkbar
+    ; `%Mkbar?.xor_
+    ]
+  ];
+  dump "";
+  trefl ()
+
+[@@postprocess_with pp']
+let test3 (x:xNxM lN.xN m) :
+  Stack (xNxM lN.xN p)
+    (requires fun _ -> True)
+    (ensures fun _ _ _ -> True)
+  =
+  test2 x
 
 let impl (lN:bar) (x:xNxM lN.xN m) : xNxM lN.xN p =
   circuit_spec2 circ lN x
 
 let spec (a:UI.uint_t m) : UI.uint_t p = a % 2
 
-let foo (lN:bar) : Lemma (
+let test1 (lN:bar) : Lemma (
   forall (x:xNxM lN.xN m) (j:nat{j<lN.xN.n}).
   column j (impl lN x) == of_uint (spec (to_uint (column j x)))
   ) =
   let impl' (x:x1xM bool m) : x1xM bool p = impl l1 x in
-  circuit_spec2_sliceable circ lN;
-  assert(sliceable (impl lN) impl');
-  assert(let i = 1 in x1xM_eq (impl' (of_uint i)) (of_uint (spec i))) by (
-    //norm [ delta_only [`%impl; `%l1; `%x1; `%Mkfoo?.t]; delta; iota; primops; simplify; nbe ];
-    norm [ delta; iota; primops; simplify; nbe ];
-    norm [ zeta; delta_only [`%circuit_spec2] ];
-    norm [ delta; iota; primops; simplify; nbe ];
-    dump "";
-    //norm [ delta; zeta; iota; primops; simplify; nbe ];
-    qed ()
+  let phi (i:UI.uint_t m) : bool = x1xM_eq (impl' (of_uint i)) (of_uint (spec i)) in
+  assert(bruteforce_aux m phi) by (
+    norm [ delta ];
+    trefl ()
   );
   admit ()
+
